boogie/binary-search-tree/insert.bpl
@@ -1,0 +1,213 @@
+// Supporting Artifact for
+// "Predictive Verification using Intrinsic Definitions of Data Structures"
+// by Adithya Murali, Cody Rivera, and P. Madhusudan.
+// 
+// Artifact by Cody Rivera, 2023. 
+//
+// Verification of BST Insert.
+
+procedure BSTInsertContract(x: Ref, k: int)
+    returns (ret: Ref);
+    requires Br == EmptyRefSet;
+    requires x != null ==> LC(C.k, C.l, C.r, C.p, 
+                                C.min, C.max, C.keys, C.repr,
+                                x);
+    requires x != null ==> !(C.keys[x])[k];
+    modifies C.k, C.l, C.r, C.p,
+        C.min, C.max, C.keys,
+        C.repr, Br, alloc;
+    ensures RefSetSubset(old(alloc), alloc);
+    ensures ret != null;
+    ensures LC(C.k, C.l, C.r, C.p, 
+                C.min, C.max, C.keys, C.repr,
+                ret);
+    ensures C.p[ret] == null;
+    ensures x != null ==> ret == x;
+    ensures (x == null ==>
+                KeySetsEqual(C.keys[ret], EmptyKeySet[k := true])
+                && C.min[ret] == k
+                && C.max[ret] == k
+                && Fresh(C.repr[ret], alloc, old(alloc))
+                && RefSetsEqual(Br, EmptyRefSet));
+    ensures (x != null ==>
+                KeySetsEqual(C.keys[ret], (old(C.keys)[x])[k := true])
+                && (C.min[ret] == old(C.min)[x] || C.min[ret] == k)
+                && (C.max[ret] == old(C.max)[x] || C.max[ret] == k)
+                && Fresh(RefSetDiffF(C.repr[ret], old(C.repr)[x]), alloc, old(alloc))
+                && (old(C.p)[x] == null ==> RefSetsEqual(Br, EmptyRefSet))
+                && (old(C.p)[x] != null ==> RefSetsEqual(Br, EmptyRefSet[old(C.p)[x] := true])));
+    // Framing conditions.
+    ensures Frame_all(
+        C.k, C.l, C.r, C.p,
+        C.min, C.max, C.keys, C.repr,
+        old(C.k), old(C.l), old(C.r), old(C.p), 
+        old(C.min), old(C.max), old(C.keys), old(C.repr),
+        if x == null then EmptyRefSet else old(C.repr)[x], old(alloc)
+    );
+
+procedure BSTInsert(x: Ref, k: int)
+    returns (ret: Ref)
+    requires Br == EmptyRefSet;
+    requires x != null ==> LC(C.k, C.l, C.r, C.p, 
+                                C.min, C.max, C.keys, C.repr,
+                                x);
+    requires x != null ==> !(C.keys[x])[k];
+    modifies C.k, C.l, C.r, C.p,
+        C.min, C.max, C.keys,
+        C.repr, Br, alloc;
+    ensures RefSetSubset(old(alloc), alloc);
+    ensures ret != null;
+    ensures LC(C.k, C.l, C.r, C.p, 
+                C.min, C.max, C.keys, C.repr,
+                ret);
+    ensures C.p[ret] == null;
+    ensures x != null ==> ret == x;
+    ensures (x == null ==>
+                KeySetsEqual(C.keys[ret], EmptyKeySet[k := true])
+                && C.min[ret] == k
+                && C.max[ret] == k
+                && Fresh(C.repr[ret], alloc, old(alloc))
+                && RefSetsEqual(Br, EmptyRefSet));
+    ensures (x != null ==>
+                KeySetsEqual(C.keys[ret], (old(C.keys)[x])[k := true])
+                && (C.min[ret] == old(C.min)[x] || C.min[ret] == k)
+                && (C.max[ret] == old(C.max)[x] || C.max[ret] == k)
+                && Fresh(RefSetDiffF(C.repr[ret], old(C.repr)[x]), alloc, old(alloc))
+                && (old(C.p)[x] == null ==> RefSetsEqual(Br, EmptyRefSet))
+                && (old(C.p)[x] != null ==> RefSetsEqual(Br, EmptyRefSet[old(C.p)[x] := true])));
+    // Framing conditions.
+    ensures Frame_all(
+        C.k, C.l, C.r, C.p,
+        C.min, C.max, C.keys, C.repr,
+        old(C.k), old(C.l), old(C.r), old(C.p), 
+        old(C.min), old(C.max), old(C.keys), old(C.repr),
+        if x == null then EmptyRefSet else old(C.repr)[x], old(alloc)
+    );
+{
+    // Local variable declarations
+    var leaf: Ref;
+    var tmp: Ref;
+    var oldl: Ref;
+    var oldr: Ref;
+
+    // Intermediate Expresssions
+    var x_k: int; var x_l: Ref; var x_r: Ref;
+    var x_l_min: int; var x_r_max: int; 
+    var x_l_keys: KeySet; var x_l_repr: RefSet;
+    var x_r_keys: KeySet; var x_r_repr: RefSet;
+
+    call InAllocParam(x);
+
+    if (x != null) {
+        call x_k := Get_k(x);
+        call x_l := Get_l(x);
+        call x_r := Get_r(x);
+    }
+    if (x == null) {
+        call leaf := Create(k);
+
+        call Set_min(leaf, k);
+        call Set_max(leaf, k);
+        call Set_keys(leaf, EmptyKeySet[k := true]);
+        call Set_repr(leaf, EmptyRefSet[leaf := true]);
+        
+        call AssertLCAndRemove(leaf);
+        ret := leaf;
+    } else if (k < x_k) {
+        call IfNotBr_ThenLC(x_l);
+        call IfNotBr_ThenLC(x_r);
+
+        call tmp := BSTInsertContract(x_l, k);
+        call x_l := Get_l(x);
+        call x_r := Get_r(x);
+        call IfNotBr_ThenLC(x_l);
+        call IfNotBr_ThenLC(x_r);
+
+        oldl := x_l;
+        call Set_l(x, tmp);
+        call Set_p(tmp, x);
+
+        call x_l := Get_l(x);
+        call x_r := Get_r(x);
+        call x_k := Get_k(x);
+        if (x_l != null) {
+            call x_l_min := Get_min(x_l);
+            call x_l_keys := Get_keys(x_l);
+            call x_l_repr := Get_repr(x_l);
+        }
+        if (x_r != null) {
+            call x_r_max := Get_max(x_r);
+            call x_r_keys := Get_keys(x_r);
+            call x_r_repr := Get_repr(x_r);
+        }
+        call Set_min(x, if x_l == null then x_k else x_l_min);
+        call Set_max(x, if x_r == null then x_k else x_r_max);
+        call Set_keys(x, 
+            KeySetUnionF(
+                (if x_l == null then EmptyKeySet else x_l_keys)[x_k := true],
+                if x_r == null then EmptyKeySet else x_r_keys
+            )
+        );
+        call Set_repr(x, 
+            RefSetUnionF(
+                (if x_l == null then EmptyRefSet else x_l_repr)[x := true],
+                if x_r == null then EmptyRefSet else x_r_repr
+            )
+        );
+        call Set_p(x, null);
+
+        call AssertLCAndRemove(tmp);
+        call AssertLCAndRemove(x);
+        call AssertLCAndRemove(oldl);
+
+        ret := x;
+    } else {
+        call IfNotBr_ThenLC(x_l);
+        call IfNotBr_ThenLC(x_r);
+
+        call tmp := BSTInsertContract(x_r, k);
+        call x_l := Get_l(x);
+        call x_r := Get_r(x);
+        call IfNotBr_ThenLC(x_l);
+        call IfNotBr_ThenLC(x_r);
+
+        oldr := x_r;
+        call Set_r(x, tmp);
+        call Set_p(tmp, x);
+
+        call x_l := Get_l(x);
+        call x_r := Get_r(x);
+        call x_k := Get_k(x);
+        if (x_l != null) {
+            call x_l_min := Get_min(x_l);
+            call x_l_keys := Get_keys(x_l);
+            call x_l_repr := Get_repr(x_l);
+        }
+        if (x_r != null) {
+            call x_r_max := Get_max(x_r);
+            call x_r_keys := Get_keys(x_r);
+            call x_r_repr := Get_repr(x_r);
+        }
+        call Set_min(x, if x_l == null then x_k else x_l_min);
+        call Set_max(x, if x_r == null then x_k else x_r_max);
+        call Set_keys(x, 
+            KeySetUnionF(
+                (if x_l == null then EmptyKeySet else x_l_keys)[x_k := true],
+                if x_r == null then EmptyKeySet else x_r_keys
+            )
+        );
+        call Set_repr(x, 
+            RefSetUnionF(
+                (if x_l == null then EmptyRefSet else x_l_repr)[x := true],
+                if x_r == null then EmptyRefSet else x_r_repr
+            )
+        );
+        call Set_p(x, null);
+
+        call AssertLCAndRemove(tmp);
+        call AssertLCAndRemove(x);
+        call AssertLCAndRemove(oldr);
+
+        ret := x;
+    }
+}
